\documentclass[11pt]{article}
\usepackage[margin=1.25in]{geometry}
\usepackage{amsmath, amssymb, enumerate, enumitem}
\usepackage{setspace}
\onehalfspacing

\begin{document}

\begin{itemize}
  \item \textbf{*Problem 9.2(g-h).} Tinker and then compute formulas that do not contain a sum for the following:
  \begin{enumerate}[label=(g)]
    \item $\displaystyle \sum_{i=1}^n ij$\\
    \begin{tabular}{l c}
      $= \displaystyle j\sum_{i=1}^n i$ & Constant Rule\\[0.25in]
      $= j \frac{n(n+1)}{2}$ & Common Sums
    \end{tabular}
  \end{enumerate}
  \begin{enumerate}[label=(h)]
    \item $\displaystyle \sum_{i=0}^n (i+j)^2$\\
    \begin{tabular}{l c}
      $= \displaystyle \sum_{i=0}^n (i^2 + 2ij + j^2)$ & Distribute \\[0.25in]
      $= \displaystyle \sum_{i=0}^n (i^2) + \displaystyle \sum_{i=0}^n (2ij) + \displaystyle \sum_{i=0}^n (j^2)$ & Addition Rule\\[0.25in]
      $= \frac{n(n+1)(2n+1)}{6} + \displaystyle \sum_{i=0}^n (2ij) + \displaystyle \sum_{i=0}^n (j^2)$ & Common Sums\\[0.25in]
      $= \frac{n(n+1)(2n+1)}{6} + 2j \displaystyle \sum_{i=0}^n i + j^2 \displaystyle \sum_{i=0}^n 1$ & Constant Rule\\[0.25in]
      $= \frac{n(n+1)(2n+1)}{6} + 2j\frac{n(n+1)}{2} + j^2(n+1)$ & Common Sums\\[0.25in]
      $= \frac{n(n+1)(2n+1)}{6} + jn(n+1) + j^2n+j^2$ & Simplify and Distribute\\[0.25in]
    \end{tabular}
  \end{enumerate}
  \item \textbf{*Problem 9.3(j-k).} Compute formulas that do not contain a sum for the following:
  \begin{enumerate}[label=(j)]
    \item $\displaystyle \sum_{i = 0}^n \displaystyle \sum_{j=0}^i 2^i$\\
    \begin{tabular}{l c}
      $= \displaystyle \sum_{i=0}^n i \displaystyle \sum_{j=0}^i 2^i$ & Innermost Sum\\[0.25in]
      $= \displaystyle \sum_{i=0}^n i (2^{i+1} - 1)$ & Common Sums \\[0.25in]
      $= \displaystyle \sum_{i=0}^n (i2^{i+1} - i)$ & Distribute \\[0.25in]
      $= \displaystyle \sum_{i=0}^n i2^{i+1} - \displaystyle \sum_{i=0}^n i$ & Addition Rule \\[0.25in]
      $= \displaystyle \sum_{i=0}^n i2^i \cdot 2^1 - \displaystyle \sum_{i=0}^n i$ & Simplify \\[0.25in]
      $= 2 \displaystyle \sum_{i=0}^n i2^i - \displaystyle \sum_{i=0}^n i$ & Constant Rule \\[0.25in]
      $= 2(\frac{n(n+1)}{2})(2^{n+1} - 1) - \frac{n(n+1)}{2}$ & Common Sums \\[0.25in]
      $= n(n+1)(2^{n+1}-1) - \frac{n(n+1)}{2}$ & Simplify \\[0.25in]
    \end{tabular}
  \end{enumerate}
  \begin{enumerate}[label=(k)]
    \item $\displaystyle \sum_{i=0}^n\sum_{j=0}^i i2^j$\\[0.25in]
    \begin{tabular}{l c}
      $= \displaystyle \sum_{i=0}^n i \displaystyle \sum_{j=0}^n 2^i$ & Innermost Sum\\[0.25in]
      $= \displaystyle \sum_{i=0}^n i(2^{i+1}-1)$ & Common Sums\\[0.25in]
      $= \displaystyle \sum_{i=0}^n i$ & The rest in ipad...
    \end{tabular}
  \end{enumerate}
  \item \textbf{*Problem 9.14.} Determine which of these functions is in $\Theta(n)$, in $\Theta(n^2)$, or neither.\\
  \begin{tabular}{c c c}
    $\Theta(n)$ & $\Theta(n^2)$ & neither \\
    b & e & a\\
    c & i & g\\
    d &   & h\\
    f &   & j\\
  \end{tabular}
  \item \textbf{*Problem 9.31(a-b).} Give the asymptotic big-Theta behavior of the runtime $T_n$, where,
  \begin{enumerate}[label=(\alph*)]
    \item $T_0 = 1$; $T_n = T_{n-1} + n^2$; for $n \geq 2$
    \begin{itemize}[label=]
      \item $\Theta(n)$
    \end{itemize}
    \item $T_0 = 1$; $T_1 = 2$; $T_n = 2T_{n-1} - T_{n-2} + 2$ for $n \geq 2$
    \begin{itemize}[label=]
      \item $\Theta(2^n)$
    \end{itemize}
  \end{enumerate}

\end{itemize}

\end{document}