\documentclass{article}
\usepackage[margin=1.25in]{geometry}
\usepackage{amsmath, amssymb, setspace, enumerate, enumitem}
\usepackage[makeroom]{cancel}
\onehalfspacing

\begin{document}
    \begin{itemize}
        \item \textbf{Problem 7.9.} $G^0 = 0$. $G_1 = 1$ and $G_n = 7G_{n-1} - 12 G_{n-2}$ for $n > 1$. Compute $G_5$. Show $G_n = 4^n - 3^n$ for $n \geq 0$.
        \item \textbf{Problem 7.12(c). (See Problem 7.28 for hints.)} Tinker to guess a formula for each recurrence and prove it. In each case $A_1 = 1$ and for $n > 1$:
        \begin{enumerate}[label=(c)]
            \item $A_n = 10nA_{n-1} / (n-1) + n$
            \newline
            \begin{tabular}{ |c|c|c|c|c| } 
                \hline
                $n$ & 2 & 3 & 4 & 5\\ 
                \hline
                $A_n$ & 22 & 333 & 4444 & 55555 \\
                \hline
            \end{tabular}
            \begin{enumerate}[label=\roman*.]
                \item formula found:
                \begin{align*}
                    \frac{10^n-1}{9}n
                \end{align*}
                \item prove the base case:
                \begin{align*}
                    A(2) &= \frac{100-1}{9}(2)\\
                         &= \frac{99}{9}(2) = 22
                \end{align*}
                \begin{center}
                    base case proven
                \end{center}

                \item prove using direct proof
                \begin{align*}
                    10n\frac{A(n-1)}{n-1} + n = \frac{10^n-1}{9}(n)
                \end{align*}
                \begin{center}
                    with with LHS
                \end{center}
                \begin{align*}
                    10n\frac{A(n-1)}{n-1} + n &= 10n \frac{\frac{10^{n-1}-1}{9}\cancel{(n-1)}}{\cancel{n-1}} + n\\
                                              &= \cancel{(10)}n(\frac{10^n - 10}{\cancel{10}}\frac{1}{9}) + n\\
                                              &= n \frac{10^n - 10}{9} + n\\
                                              &= n \frac{10^n - 10}{9} + \frac{9n}{9}\\
                                              &= \frac{10^nn - 10n + 9n}{9}\\
                                              &= \frac{10^nn - n}{9}\\
                            \frac{10^n-1}{9}n &= \frac{10^n-1}{9}n
                \end{align*}
                \item we prove by direct proof that the statement is true for all $n > 1$ $\hfill \blacksquare$
            \end{enumerate}
        \end{enumerate}
        \item \textbf{Problem 7.13(a).} Analyze these very fast growing recursions. [Hint: Take logarithms.]
        \begin{enumerate}[label=(a)]
            \item $M_1 = 2$ and $M_n = aM^2_{n-1}$ for $n>1$. Guess and prove a formula for $M_n$. Tinker, tinker.
            \begin{tabular}{ |c|c|c|c|c| } 
                \hline
                $n$ & 2 & 3 & 4 & 5\\ 
                \hline
                $A_n$ & a4 & a16 & a256 & a65536 \\
                \hline
            \end{tabular}
            \begin{enumerate}[label=(\roman*)]
                \item formula found:
                \begin{align*}
                    M(n) = 2^{2^{n-1}}\\
                \end{align*}
                \item base case:
                \begin{align*}
                    M(2) &= a(2^{2^1})\\
                         &= a(2^2)\\
                         &= a4
                \end{align*}
                \begin{center}
                    base case proven
                \end{center}
                \item prove using direct proof
                \begin{align*}
                    aM(n-1)^2 &= a2^{2^{n-1}}\\
                    M(n-1)^2 &= 2^{2^{n-1}} \text{ simplify}\\
                    \log_{2}(M(n-1)^2) &= \log_2(2^{2^{n-1}}) \text{ log both sides}\\
                    \log_{2}(M(n-1)^2) &= 2^{2^{n-1}}\\
                \end{align*}
                \begin{center}
                    work with LHS
                \end{center}
                \begin{align*}
                    \log_{2}(M(n-1)^2) & = 2 \log_{2}(M(n-1))\\
                                       & = 2 \log_{2}(2^{2^{(n-1) - 1}})\\
                                       & = 2(2^{n-2})\\
                                       & = 2^{n-1}
                \end{align*}
                \item we prove by direct proof that the statement is true for all $n > 1$ $\hfill\blacksquare$
            \end{enumerate}
        \end{enumerate}
        \item \textbf{Problem 7.19(d).} Recall the Fibonacci numbers: $F_1$, $F_2 = 1$; and, $F_n = F_{n-1} + F_{n-2}$ for $n > 2$
        \begin{enumerate}[label=(d)]
            \item Prove that every third Fibonacci number, $F_{3n}$, is even
        \end{enumerate}
        \item \textbf{Problem 7.42.}
        \item \textbf{Problem 7.45(c).}
        \item \textbf{Problem 7.49.}
        \item \textbf{Problem 8.12(d).}
        \item \textbf{Problem 8.14.}
    \end{itemize}
    
\end{document}